do not overwrite code of existing accounts

Hoare/Invariants.thy
@@ -130,9 +130,182 @@ by (auto simp add:next0_def Let_def
    contract_action.split_asm stack_hint.split_asm
    instruction_result.splits)
 
+lemma can_exit :
+  "Finished st2 = next0 net (Continue st1) \<Longrightarrow>
+   length (g_stack st1) = 0 \<or>
+   length (g_stack st1) = 1 \<and> g_create st1"
+by (auto simp add:next0_def Let_def
+  split:if_split_asm option.split_asm list.split_asm
+   contract_action.split_asm stack_hint.split_asm
+   instruction_result.splits)
+
+lemma create_const :
+  "Continue st2 = next0 net (Continue st1) \<Longrightarrow>
+   g_create st1 = g_create st2"
+by (auto simp add:next0_def Let_def
+  split:if_split_asm option.split_asm list.split_asm
+   contract_action.split_asm stack_hint.split_asm
+   instruction_result.splits)
+
+
 (* code changes *)
+lemma code_return :
+  "account_code0 (update_return st1 addr2 x32 addr) =
+   account_code0 (st1 addr)"
+by (auto simp add:update_return_def update_world_def)
+
+lemma code_call :
+  "account_code0 (update_call st1 addr2 x32 addr) =
+   account_code0 (st1 addr)"
+by (auto simp add:update_call_def transfer_balance_def
+   add_balance_def sub_balance_def Let_def update_world_def)
+
+lemma code_transfer :
+  "account_code0 (transfer_balance st1 addr2 x32 v addr) =
+   account_code0 (st1 addr)"
+by (auto simp add:update_call_def transfer_balance_def
+   add_balance_def sub_balance_def Let_def update_world_def)
+
+lemma code_update :
+  "account_code0 (update_world st1 addr2 acc addr) =
+   ( if addr2 = addr then account_code0 acc
+     else account_code0 (st1 addr))"
+by (auto simp add:update_call_def transfer_balance_def
+   add_balance_def sub_balance_def Let_def update_world_def)
+
+lemma code_nonce :
+  "account_code0 (update_nonce st1 addr2 addr) =
+   account_code0 (st1 addr)"
+by (auto simp add:update_nonce_def transfer_balance_def
+   add_balance_def sub_balance_def Let_def update_world_def)
+
+lemma code_stay :
+  "Continue st2 = next0 net (Continue st1) \<Longrightarrow>
+   g_stack st2 = g_stack st1 \<Longrightarrow>
+   account_code0 (g_current st1 addr) =
+   account_code0 (g_current st2 addr)"
+by (auto simp add:next0_def Let_def
+  code_return
+  split:if_split_asm option.split_asm list.split_asm
+   contract_action.split_asm stack_hint.split_asm
+   instruction_result.splits)
+
+lemma weird : 
+   "g_current st2 = a \<Longrightarrow>
+    account_code0 (a addr) = account_code0 (g_current st2 addr)"
+by auto
+
+lemma weird2 :
+ "st2 = st1
+    \<lparr>g_stack := d, g_current := a,
+       g_cctx := c,
+       g_vmstate := e \<rparr> \<Longrightarrow>
+  g_current st2 = a"
+by auto
+
+(* separate cases for fail etc. *)
+lemma code_fail :
+  "Continue st2 = next0 net (Continue st1) \<Longrightarrow>
+   g_vmstate st1 = InstructionToEnvironment (ContractFail lst) v1 hint \<Longrightarrow>
+   (a,b,c,d) # g_stack st2 = g_stack st1 \<Longrightarrow>
+   account_code0 (a addr) =
+   account_code0 (g_current st2 addr)"
+by (auto simp add:next0_def Let_def
+  code_return
+  split:if_split_asm option.split_asm list.split_asm
+   contract_action.split_asm stack_hint.split_asm
+   instruction_result.splits)
+
+fun stack_hint :: "world_state * variable_ctx * constant_ctx * stack_hint \<Rightarrow> stack_hint" where
+"stack_hint (a,b,c,d) = d"
+
+fun stack_state :: "world_state * variable_ctx * constant_ctx * stack_hint \<Rightarrow> world_state" where
+"stack_state (a,b,c,d) = a"
+
+lemma code_suicide :
+  "next0 net (Continue st1) = Continue st2 \<Longrightarrow>
+   g_vmstate st1 = InstructionToEnvironment (ContractSuicide lst) v1 hint \<Longrightarrow>
+   stack_hint (hd (g_stack st1)) \<noteq> CreateAddress addr \<Longrightarrow>
+   account_code0 (g_current st1 addr) =
+   account_code0 (g_current st2 addr)"
+by (auto simp add:next0_def Let_def
+  code_return code_update create_account_def
+  split:if_split_asm option.split_asm list.split_asm
+   contract_action.split_asm stack_hint.split_asm
+   instruction_result.splits)
+
+lemma code_ret :
+  "next0 net (Continue st1) = Continue st2 \<Longrightarrow>
+   g_vmstate st1 = InstructionToEnvironment (ContractReturn lst) v1 hint \<Longrightarrow>
+   stack_hint (hd (g_stack st1)) \<noteq> CreateAddress addr \<Longrightarrow>
+   account_code0 (g_current st2 addr) =
+   account_code0 (g_current st1 addr) \<or>
+   account_code0 (g_current st2 addr) =
+   account_code0 (stack_state (hd (g_stack st1)) addr)"
+by (auto simp add:next0_def Let_def
+  code_return code_update create_account_def
+  split:if_split_asm option.split_asm list.split_asm
+   contract_action.split_asm stack_hint.split_asm
+   instruction_result.splits)
+
+
+(* in the hypotheses, matters a lot if it is a=b or b=a *)
+lemma code_push :
+  "Continue st2 = next0 net (Continue st1) \<Longrightarrow>
+   tl (g_stack st2) = g_stack st1 \<Longrightarrow>
+   account_exists (g_current st1 addr) \<Longrightarrow>
+   account_code0 (g_current st1 addr) =
+   account_code0 (g_current st2 addr)"
+by (auto simp add:next0_def Let_def
+  code_return code_call code_transfer code_update tl_wf
+  code_nonce
+  split:if_split_asm option.split_asm list.split_asm
+   contract_action.split_asm stack_hint.split_asm
+   instruction_result.splits)
+
+lemma push_create_hint :
+  "Continue st2 = next0 net (Continue st1) \<Longrightarrow>
+   g_stack st2 = abcd # g_stack st1 \<Longrightarrow>
+   stack_hint abcd = CreateAddress addr \<Longrightarrow>
+   account_exists (g_current st1 addr) \<Longrightarrow>
+   False"
+by (auto simp add:next0_def Let_def
+  code_return code_call
+  code_transfer code_update tl_wf
+  code_nonce get_hint_def
+  split:if_split_asm option.split_asm list.split_asm
+   contract_action.split_asm stack_hint.split_asm
+   instruction_result.splits)
+
+definition first_return :: "network \<Rightarrow> global0 \<Rightarrow> nat \<Rightarrow> bool" where
+"first_return net st k = (
+   iter_next net (Continue st) k = Unimplemented \<or>
+   (\<exists>st2. Continue st2 = iter_next net (Continue st) k \<and>
+          tl (g_stack st) = g_stack st2 \<and>
+    (\<forall>l<k. \<forall>st3. Continue st3 = iter_next net (Continue st) l \<longrightarrow>
+                 tl (g_stack st) \<noteq> g_stack st3)))"
+
+(* account existence continues until first return *)
+
+lemma exist_until_return :
+  "account_exists (g_current st1 addr) \<Longrightarrow>
+   first_return net st1 k \<Longrightarrow>
+   l < k \<Longrightarrow>
+   Continue st3 = iter_next net (Continue st) l \<Longrightarrow>
+   account_exists (g_current st3 addr)"
 
 (* storage changes *)
+(* storage changes are first the same as code changes, but also from
+   calls out *)
+lemma storage_continue :
+  "Continue st2 = next0 net (Continue st1) \<Longrightarrow>
+   g_vmstate st1 \<in> range InstructionContinue \<Longrightarrow>
+   account_storage0 (g_current st1 addr) =
+   account_storage0 (g_current st2 addr)"
+by (auto simp add:next0_def Let_def
+  split:if_split_asm option.split_asm list.split_asm
+   contract_action.split_asm stack_hint.split_asm
+   instruction_result.splits)
 
 (* balance changes *)
 
